src/program_proof/simplepb/apps/closed_proof.v
@@ -1,0 +1,97 @@
+From Perennial.program_proof Require Import grove_prelude.
+From Goose.github_com.mit_pdos.gokv.simplepb.apps Require Import closed.
+
+From Perennial.goose_lang Require adequacy dist_adequacy.
+From Perennial.goose_lang.ffi Require grove_ffi_adequacy.
+From Perennial.program_logic Require dist_lang.
+
+From Perennial.program_proof.simplepb Require Import config_proof.
+From Perennial.program_proof.grove_shared Require Import urpc_proof.
+
+Module closed.
+
+Import adequacy dist_adequacy grove_ffi_adequacy dist_lang.
+
+Definition grove_dist_adequate
+           (enonidempσs: list (node_init_cfg (Λ:=goose_lang)))
+           (ebσs: list (goose_lang.expr * goose_lang.state))
+           (g: goose_lang.global_state) :=
+  let ρs := fmap (λ ebσ, {| init_thread := fst ebσ;
+                           init_restart := fst ebσ;
+                           init_local_state := snd ebσ |})
+               ebσs in
+  dist_adequacy.dist_adequate (CS := goose_crash_lang) (enonidempσs ++ ρs) g.
+
+Definition kv_pbΣ := #[heapΣ; mono_natΣ; ghost_varΣ (list u64); urpcregΣ].
+
+Definition configHost : chan := U64 10.
+
+Lemma kv_pb_boot :
+  ∀ σconfig σsrv1 σsrv2 (g : goose_lang.global_state),
+  (* *)
+  ffi_initgP g.(global_world) →
+
+  ffi_initP σconfig.(world) g.(global_world) →
+  ffi_initP σsrv1.(world) g.(global_world) →
+  ffi_initP σsrv2.(world) g.(global_world) →
+  (*
+  g.(global_world).(grove_net) !! shardId = Some (∅ : gset message) →
+  g.(global_world).(grove_net) !! coordId = Some (∅ : gset message) → *)
+  grove_dist_adequate
+    [ {| init_thread := config_main #() ; init_restart := of_val #(); init_local_state := σconfig |}]
+    [(kv_replica_main1 #(), σsrv1); (kv_replica_main2 #(), σsrv2)] g (λ _, True).
+Proof.
+  intros ????.
+  intros Hinitg Hinitconfig Hinitr1 Hinitr2.
+  eapply (grove_ffi_dist_adequacy (kv_pbΣ)).
+  { assumption. }
+  { repeat constructor; naive_solver. }
+
+  intros Hheap.
+  iIntros "Hchan".
+  iSplitR ""; last first.
+  { iModIntro. iMod (fupd_mask_subseteq ∅); eauto. }
+
+  (* TODO: initialize ghost state, including RPC stuff *)
+
+  iMod (config_ghost_init) as (γconf) "HconfInit".
+  iMod (config_server_init configHost γconf with "[]") as "#HisConf".
+  { admit. }
+
+  iModIntro.
+  simpl. iSplitL "HconfInit".
+  {
+    iIntros (HL) "Hfiles".
+    iModIntro.
+    iExists (λ _, True%I), (λ _, True%I), (λ _ _, True%I).
+    set (hG' := HeapGS _ _ _). (* overcome impedence mismatch between heapGS (bundled) and gooseGLobalGS+gooseLocalGS (split) proofs *)
+    iApply (idempotence_wpr with "[HconfInit] []").
+    {
+      instantiate (1:=λ _, True%I).
+      simpl.
+      iApply wp_wpc.
+      wp_call.
+      iDestruct "HconfInit" as "(H1 & H2 & _)".
+      wp_apply (config_proof.wp_MakeServer with "[H1 H2]").
+      {
+        iFrame.
+      }
+      iIntros (?) "#Hisconf_server".
+      wp_apply (config_proof.wp_Server__Serve with "[$]").
+      { iFrame "#". }
+      wp_pures.
+      by iModIntro.
+    }
+    { (* crash; there should actually be no crashes *)
+      iModIntro.
+      iIntros.
+      iModIntro.
+      admit.
+    }
+  }
+  (* other servers remain *)
+Admitted.
+
+Print Assumptions kv_pb_boot.
+
+End closed.
